src/opt/ReorderUpdate.v
@@ -1,0 +1,232 @@
+Require Import Basics.
+Require Import Bool.
+Require Import List.
+
+Require Import sflib.
+Require Import paco.
+Require Import respectful5.
+
+Require Import Basic.
+Require Import Event.
+Require Import Language.
+Require Import Time.
+Require Import Memory.
+Require Import Commit.
+Require Import Thread.
+
+Require Import Configuration.
+Require Import Simulation.
+Require Import Compatibility.
+Require Import MemInv.
+Require Import ReorderBase.
+
+Require Import Syntax.
+Require Import Semantics.
+
+Set Implicit Arguments.
+
+
+Inductive reorder_update r1 l1 rmw1 o1: forall (i2:Instr.t), Prop :=
+| reorder_update_load
+    r2 l2 o2
+    (ORD1: Ordering.le o1 Ordering.relaxed)
+    (ORD2: Ordering.le o2 Ordering.release)
+    (LOC: l1 <> l2)
+    (REGS: RegSet.disjoint (Instr.regs_of (Instr.update r1 l1 rmw1 o1))
+                           (Instr.regs_of (Instr.load r2 l2 o2))):
+    reorder_update r1 l1 rmw1 o1 (Instr.load r2 l2 o2)
+| reorder_update_store
+    l2 v2 o2
+    (ORD1: Ordering.le o1 Ordering.relaxed)
+    (LOC: l1 <> l2)
+    (REGS: RegSet.disjoint (Instr.regs_of (Instr.update r1 l1 rmw1 o1))
+                           (Instr.regs_of (Instr.store l2 v2 o2))):
+    reorder_update r1 l1 rmw1 o1 (Instr.store l2 v2 o2)
+| reorder_update_update
+    r2 l2 rmw2 o2
+    (ORD1: Ordering.le o1 Ordering.relaxed)
+    (ORD2: Ordering.le o2 Ordering.release)
+    (LOC: l1 <> l2)
+    (REGS: RegSet.disjoint (Instr.regs_of (Instr.update r1 l1 rmw1 o1))
+                           (Instr.regs_of (Instr.update r2 l2 rmw2 o2))):
+    reorder_update r1 l1 rmw1 o1 (Instr.update r2 l2 rmw2 o2)
+.
+
+Inductive sim_update: forall (st_src:lang.(Language.state)) (th_src:Local.t) (mem_k_src:Memory.t)
+                        (st_tgt:lang.(Language.state)) (th_tgt:Local.t) (mem_k_tgt:Memory.t), Prop :=
+| sim_update_intro
+    r1 l1 from1 to1 vr1 vret1 vw1 releasedr1 releasedw1 rmw1 o1 i2
+    rs th1_src th1_tgt th2_src th3_src
+    mem_k_src mem_k_tgt
+    (REORDER: reorder_update r1 l1 rmw1 o1 i2)
+    (RMW: RegFile.eval_rmw rs rmw1 vr1 = (vret1, vw1))
+    (READ: Local.read_step th1_src mem_k_src l1 from1 vr1 releasedr1 o1 th2_src)
+    (FULFILL: Local.fulfill_step th2_src mem_k_src l1 from1 to1 vw1 releasedw1 o1 th3_src)
+    (RELEASED: Snapshot.le releasedr1 releasedw1)
+    (LOCAL: sim_local th3_src th1_tgt):
+    sim_update
+      (State.mk rs [Stmt.instr i2; Stmt.instr (Instr.update r1 l1 rmw1 o1)]) th1_src mem_k_src
+      (State.mk (RegFun.add r1 vret1 rs) [Stmt.instr i2]) th1_tgt mem_k_tgt
+.
+
+Lemma sim_update_sim_thread:
+  sim_update <6= (sim_thread (sim_terminal eq)).
+Proof.
+  pcofix CIH. i. pfold. ii. ss. splits; ss.
+  - i. inv TERMINAL_TGT. inv PR; ss.
+  - admit.
+    (* future; https://github.com/jeehoonkang/memory-model-explorer/blob/86c803103989f87a17f50e6349aa9f285104af09/formalization/src/opt/Reorder.v#L100 *)
+  - admit.
+  - inv PR. i. inv STEP_TGT; [|by inv STEP; inv STATE; inv INSTR; inv REORDER].
+    exploit Local.future_read_step; try apply READ; eauto. i.
+    exploit Local.future_fulfill_step; try apply FULFILL; eauto. i.
+    inv STEP; try (inv STATE; inv INSTR; inv REORDER); ss.
+    + (* promise *)
+      exploit sim_local_promise; eauto.
+      { eapply Local.fulfill_step_future; eauto.
+        eapply Local.read_step_future; eauto.
+      }
+      i. des.
+      exploit reorder_fulfill_promise; try apply x3; try apply STEP_SRC; eauto.
+      { eapply Local.read_step_future; eauto. }
+      i. des.
+      exploit reorder_read_promise; try apply x0; try apply STEP1; eauto. i. des.
+      exploit sim_local_fulfill; try apply LOCAL3; try reflexivity; eauto.
+      { eapply Local.read_step_future; eauto.
+        eapply Local.promise_step_future; eauto.
+      }
+      { eapply Local.promise_step_future; eauto.
+        eapply Local.read_step_future; eauto.
+      }
+      i. des.
+      eexists _, _, _, _, _, _. splits; eauto.
+      * econs. econs 1; eauto.
+      * right. apply CIH. econs; try apply STEP3; try apply STEP_SRC0; eauto.
+        etransitivity; eauto. etransitivity; eauto.
+    + (* load *)
+      exploit sim_local_read; eauto.
+      { eapply Local.fulfill_step_future; eauto.
+        eapply Local.read_step_future; eauto.
+      }
+      i. des.
+      exploit reorder_fulfill_read; try apply x3; try apply STEP_SRC; eauto.
+      { destruct o1; ss. }
+      { eapply Local.read_step_future; eauto. }
+      i. des.
+      exploit reorder_read_read; try apply x0; try apply STEP1; eauto. i. des.
+      exploit sim_local_fulfill; try apply SIM0; try reflexivity; eauto.
+      { eapply Local.read_step_future; eauto.
+        eapply Local.read_step_future; eauto.
+      }
+      { eapply Local.read_step_future; eauto.
+        eapply Local.read_step_future; eauto.
+      }
+      i. des.
+      eexists _, _, _, _, _, _. splits.
+      * econs 2; [|econs 1]. econs 3; eauto. econs. econs.
+      * econs. econs 5; eauto.
+        { econs. econs. erewrite RegFile.eq_except_rmw; eauto.
+          - admit.
+          - apply RegFile.eq_except_singleton.
+        }
+        { s. econs 1. eauto. }
+      * s. eauto.
+      * s. left. eapply paco7_mon; [apply sim_stmts_nil|]; ss.
+        { apply RegFun.add_add. admit. }
+        { etransitivity; eauto. etransitivity; eauto. }
+    + (* store *)
+      exploit sim_local_write; eauto.
+      { eapply Local.fulfill_step_future; eauto.
+        eapply Local.read_step_future; eauto.
+      }
+      i. des.
+      exploit reorder_fulfill_write; try apply x3; try apply STEP_SRC; eauto.
+      { destruct o1; ss. }
+      { eapply Local.read_step_future; eauto. }
+      i. des.
+      exploit reorder_read_write; try apply x0; try apply STEP1; eauto.
+      { destruct o1; ss. }
+      i. des.
+      exploit sim_local_fulfill; try apply SIM0; try reflexivity; eauto.
+      { eapply Local.read_step_future; eauto.
+        eapply Local.write_step_future; eauto.
+      }
+      { eapply Local.write_step_future; eauto.
+        eapply Local.read_step_future; eauto.
+      }
+      i. des.
+      eexists _, _, _, _, _, _. splits.
+      * econs 2; [|econs 1]. econs 4; eauto. econs.
+        erewrite <- RegFile.eq_except_value; eauto.
+        { econs. }
+        { admit. }
+      * econs. econs 5; eauto.
+        { econs. econs. eauto. }
+        { s. econs 1. eauto. }
+      * s. eauto.
+      * s. left. eapply paco7_mon; [apply sim_stmts_nil|]; ss.
+        etransitivity; eauto. etransitivity; eauto.
+    + (* update *)
+      exploit sim_local_read; eauto.
+      { eapply Local.fulfill_step_future; eauto.
+        eapply Local.read_step_future; eauto.
+      }
+      i. des.
+      exploit reorder_fulfill_read; try apply x3; try apply STEP_SRC; eauto.
+      { destruct o1; ss. }
+      { eapply Local.read_step_future; eauto. }
+      i. des.
+      exploit reorder_read_read; try apply x0; try apply STEP1; eauto. i. des.
+      exploit sim_local_fulfill; try apply STEP2; try apply SIM0; try reflexivity; eauto.
+      { eapply Local.read_step_future; eauto.
+        eapply Local.read_step_future; eauto.
+      }
+      { eapply Local.read_step_future; eauto.
+        eapply Local.read_step_future; eauto.
+      }
+      i. des.
+      rewrite SIM, LOCAL0 in LOCAL3.
+      exploit sim_local_write; eauto.
+      { eapply Local.fulfill_step_future; eauto.
+        eapply Local.read_step_future; eauto.
+        eapply Local.read_step_future; eauto.
+      }
+      { eapply Local.read_step_future; eauto. }
+      i. des.
+      exploit reorder_fulfill_write; try apply STEP_SRC0; try apply STEP_SRC1; eauto.
+      { destruct o1; ss. }
+      { eapply Local.read_step_future; eauto.
+        eapply Local.read_step_future; eauto.
+      }
+      i. des.
+      exploit reorder_read_write; try apply STEP3; try apply STEP4; eauto.
+      { destruct o1; ss. }
+      { eapply Local.read_step_future; eauto. }
+      i. des.
+      exploit sim_local_fulfill; try apply STEP5; try apply SIM2; try reflexivity; eauto.
+      { eapply Local.read_step_future; eauto.
+        eapply Local.write_step_future; eauto.
+        eapply Local.read_step_future; eauto.
+      }
+      { eapply Local.write_step_future; eauto.
+        eapply Local.read_step_future; eauto.
+        eapply Local.read_step_future; eauto.
+      }
+      i. des.
+      eexists _, _, _, _, _, _. splits.
+      * econs 2; [|econs 1]. econs 5; eauto. econs. econs.
+        erewrite <- RegFile.eq_except_rmw; eauto.
+        { admit. }
+        { apply RegFile.eq_except_singleton. }
+      * econs. econs 5; try apply STEP7; try apply STEP_SRC2; eauto.
+        { econs. econs.
+          erewrite RegFile.eq_except_rmw; eauto.
+          - admit.
+          - apply RegFile.eq_except_singleton.
+        }
+        { econs 1. eauto. }
+      * eauto.
+      * left. eapply paco7_mon; [apply sim_stmts_nil|]; ss.
+        { apply RegFun.add_add. admit. }
+        { etransitivity; eauto. etransitivity; eauto. }
+Admitted.
